begin proving exp1.c

examples/compcert/experiment1/exp1.c
@@ -2,10 +2,16 @@
 // 22/6/18
 //tiny program for use in the VST
 
-int main(int argc, char* argv[])
+const int mySum(int x, int y)
+{
+    const int z = x + y;
+    return z;
+}
+
+int main(void)
 {
     const int A = 2;
     const int B = 3;
-    const int C = A + B;
+    const int C = mySum( A, B );
     return C;
 }
