examples/compcert/experiment1/verif_exp1.v
@@ -4,10 +4,86 @@ Require Import exp1. (* Import the AST of this C program *)
 Instance CompSpecs : compspecs. make_compspecs prog. Defined. 
 Definition Vprog : varspecs.  mk_varspecs prog. Defined. 
 
-
 (* Functional spec of this program.  *)
-Definition sum_Z : list Z -> Z := fold_right Z.add 0.
+Definition myAdd : Z -> Z -> Z := Z.add.
 
-Definition nameHere : int -> int -> int := add.
+Lemma assoc : forall a b c : Z, (a+(b+c)) = (a+b+c).
+Proof.
+  intuition.
+Qed.
 
+Lemma hasIdent : forall a : Z, a+0=a /\ 0+a=a.
+Proof.
+  intuition.
+Qed.
+
+Lemma hasInverse: forall a:Z, exists b:Z, a+b=0.
+Proof.
+  intros a.
+  exists (0-a).
+  intuition.
+Qed.
+
+(* Beginning of the API spec for the sumarray.c program *)
+Definition exp1_spec : ident * funspec :=
+ DECLARE _mySum
+  WITH x:val, y:val, sh : share, sum : Z
+  PRE [ _x OF tint, _y OF tint ]
+          PROP  (readable_share sh;
+                 0 <= sum <= Int.max_signed)
+          LOCAL (temp _x x; temp _y y)
+          SEP   (data_at sh (tint) (Vint (Int.repr sum)) x)
+  POST [ tint ]
+        PROP () LOCAL(temp ret_temp  (Vint (Int.repr (sum))))
+           SEP (data_at sh (tint) (Vint (Int.repr sum)) x).
+
+
+(* The precondition of "int main(void){}" always looks like this. *)
+Definition main_spec :=
+ DECLARE _main
+  WITH gv : globals
+  PRE  [] main_pre prog nil gv
+  POST [ tint ]  
+     PROP() 
+     LOCAL (temp ret_temp (Vint (Int.repr (2+3)))) 
+     SEP(TT).
+
+
+(* Packaging the API spec all together. *)
+Definition Gprog : funspecs :=
+        ltac:(with_library prog [exp1_spec; main_spec]).
+
+
+(** Proof that f_sumarray, the body of the sumarray() function,
+ ** satisfies sumarray_spec, in the global context (Vprog,Gprog).
+ **)
+Lemma body_sumarray: semax_body Vprog Gprog f_mySum exp1_spec.
+Proof.
+start_function. (* Always do this at the beginning of a semax_body proof *)
+(* The next two lines do forward symbolic execution through
+   the first two executable statements of the function body *)
+forward.
+forward.
+Qed.
+
+Lemma body_main:  semax_body Vprog Gprog f_main main_spec.
+Proof.
+start_function.
+forward.
+forward.
+forward_call (*  s = sumarray(four,4); *)
+  (Vint (Int.repr 2), Vint (Int.repr 3) ,5).
+ split3. auto. computable. repeat constructor; computable.
+forward. (* return s; *)
+Qed.
+
+Existing Instance NullExtension.Espec.
+
+Lemma prog_correct:
+  semax_prog prog Vprog Gprog.
+Proof.
+prove_semax_prog.
+semax_func_cons body_sumarray.
+semax_func_cons body_main.
+Qed.
 
